src/program_proof/tulip/program/tuple/res.v
@@ -6,4 +6,18 @@ Section res.
 
   Definition own_phys_hist_half α (key : string) (hist : dbhist) : iProp Σ.
   Admitted.
+
+  Lemma phys_hist_update {α k h1 h2} h :
+    own_phys_hist_half α k h1 -∗
+    own_phys_hist_half α k h2 ==∗
+    own_phys_hist_half α k h ∗
+    own_phys_hist_half α k h.
+  Admitted.
+
+  Lemma phys_hist_agree α k h1 h2 :
+    own_phys_hist_half α k h1 -∗
+    own_phys_hist_half α k h2 -∗
+    ⌜h2 = h1⌝.
+  Admitted.
+
 End res.
